Verbatim/actions/impl.v
@@ -2,6 +2,8 @@ From Verbatim Require Import state.
 Require Import List.
 Import ListNotations.
 
+Require Import Coq.omega.Omega.
+
 From Verbatim Require Import ltac.
 
 
@@ -38,6 +40,7 @@ Module Type SEM_USER (Import STT : state.T).
   Parameter label_carries : forall l l' s t,
       apply_sem (l, s) = Some (existT _ l' t)
       -> l = l'.
+  Parameter defLiteral : sem_ty defLabel.
 
 End SEM_USER.
 
@@ -47,41 +50,22 @@ Module SemLexerFn (STT : state.T) (Export LXR : LEXER STT) (Import USER : SEM_US
   Module Import Core.
     
     Definition sem_token := {l : Label & sem_ty l}.
+    Definition defSemToken := (existT sem_ty defLabel defLiteral).
 
   End Core. 
 
   Module Import Spec.
-      
-    Inductive tokenized_sem' (rus : list Rule) : String -> (list (option sem_token))
-                                                -> String -> Prop :=
-    | Tkd_sem'_Nil (code : String)
-               (H : tokenized rus code [] code)
-      : tokenized_sem' rus code [] code
-    | Tkd_sem'_Cons (t : option sem_token) (ts : list (option sem_token))
-               (l : Label) (p : Prefix) (s0 s1 : Suffix)
-               (Hsem : apply_sem (l, p) = t)
-               (* the first token matches the input *)
-               (H0 : first_token (p ++ s0 ++ s1) rus (l,p))
-               (* The rest of the tokens match the rest of the input *)
-               (IH : tokenized_sem' rus (s0 ++ s1) ts s1) :
-        tokenized_sem' rus (p ++ s0 ++ s1) (t :: ts) s1.
-      
-
+  
     Inductive tokenized_sem (rus : list Rule) : String -> (option (list sem_token))
                                                 -> String -> Prop :=
-      (* The Some case really needs some work  *)
     | Tkd_sem_Some (code rest : String) (ts : list Token) (sts : list sem_token)
-                   (n : nat) (st st' : sem_token) (t : Token)
                    (H0 : tokenized rus code ts rest)
-                   (H3 : (nth_error ts n = Some t
-                         /\ nth_error sts n = Some st)
-                         -> (apply_sem t = Some st' /\ st = st'))
-                   (H6 : length ts = length sts)
+                   (H1 : length ts = length sts)
+                   (H2 : forall t st,  In (t, st) (combine ts sts) -> apply_sem t = Some st)
       : tokenized_sem rus code (Some sts) rest
-    | Tkd_sem_None (code rest : String) (t : Token) (ts : list Token)
+    | Tkd_sem_None (code rest : String) (ts : list Token)
         (H : tokenized rus code ts rest)
-        (Hin : In t ts)
-        (Hsem : apply_sem t = None)
+        (Hin : exists t, In t ts /\ apply_sem t = None)
       : tokenized_sem rus code None rest.
     
   End Spec.
@@ -111,19 +95,163 @@ Module SemLexerFn (STT : state.T) (Export LXR : LEXER STT) (Import USER : SEM_US
 
   End Impl.
 
+  Module Import Lemmas.
+    
+    Lemma lo2ol_None : forall {T : Type} (xs : list (option T)),
+      lo2ol xs = None
+      <-> In None xs.
+    Proof.
+      intros; split; intros.
+      {
+        induction xs.
+        - sis. discriminate.
+        - sis. repeat dm. discriminate.
+      }
+      {
+        induction xs.
+        - sis. contradiction.
+        - sis. repeat dm. destruct H.
+          + discriminate.
+          + apply IHxs in H. discriminate.
+      }
+    Qed.
+
+    Lemma lo2ol_tail : forall {T : Type} (ys : list T) (xs : list (option T)) x y,
+        lo2ol (x :: xs) = Some (y :: ys)
+        -> lo2ol xs = Some ys.
+    Proof.
+      destruct xs; intros.
+      {
+        sis. repeat dm.
+        - repeat inj_all. auto.
+        - discriminate.
+      }
+      {
+        sis. repeat dm; repeat inj_all; auto; try discriminate.
+      }
+    Qed.
+
+    Lemma lo2ol_head : forall {T : Type} (ys : list T) (xs : list (option T)) x y,
+        lo2ol (x :: xs) = Some (y :: ys)
+        -> x = Some y.
+    Proof.
+      intros. sis. repeat dm.
+      - repeat inj_all. auto.
+      - discriminate.
+      - discriminate.
+    Qed.
+       
+    Lemma lo2ol_length : forall {T : Type} (xs : list (option T)) (ys : list T),
+      lo2ol xs = Some ys
+      -> length xs = length ys.
+    Proof.
+      induction xs; intros.
+      {
+        sis. inv H. auto.
+      }
+      {
+        destruct ys.
+        - sis. repeat dm; repeat inj_all; discriminate.
+        - apply lo2ol_tail in H. apply IHxs in H. sis. omega.
+      }
+    Qed.
+
+    (* this could be more general *)
+    Lemma lo2ol_map : forall l1 l0 l t st,
+        map apply_sem l1 = l0
+        -> lo2ol l0 = Some l
+        -> In (t, st) (combine l1 l)
+        -> apply_sem t = Some st.
+    Proof.
+      induction l1; intros.
+      {
+        sis. contradiction.
+      }
+      {
+        destruct l0. sis. discriminate. destruct l. sis. repeat dm; discriminate.
+        destruct H1.
+        - repeat inj_all. rewrite map_cons in H. injection H; intros.
+          rewrite H2. apply lo2ol_head in H0. auto.
+        - eapply IHl1; eauto.
+          rewrite <- H in H0. eapply lo2ol_tail; eauto.
+      }
+    Qed.
+
+  End Lemmas.
+
   Module Correct.
+
 
     Theorem lex_sem_sound : forall o code rest rus,
       lex_sem rus code = (o, rest)
       -> rules_is_function rus
       -> tokenized_sem rus code o rest.
     Proof.
-      intros. destruct o.
+      intros.
+      unfold lex_sem in *. repeat dm. unfold lex_sem' in *. repeat dm.
+      assert(tokenized rus code l0 rest).
       {
-        unfold lex_sem in *. unfold lex_sem' in *. repeat dm. repeat inj_all.
+        repeat inj_all. eapply lex_sound; eauto.
+      }
+      destruct o.
+      {
         eapply Tkd_sem_Some; eauto.
-        - eapply lex_sound; eauto.
-        - Abort.
+        - repeat inj_all. apply lo2ol_length in H3. rewrite map_length in H3. auto.
+        - intros. eapply lo2ol_map; eauto. repeat inj_all. auto.
+      }
+      {
+        eapply Tkd_sem_None; eauto.
+        repeat inj_all. apply lo2ol_None in H3.
+        apply in_map_iff in H3. destruct H3. exists x.
+        destruct H. split; auto.
+      }
+    Qed.
+
+    Theorem tokenized_sem_unique : forall rus code o rest o0 s,
+        tokenized_sem rus code o rest
+        -> rules_is_function rus
+        -> tokenized_sem rus code o0 s
+        -> (o, rest) = (o0, s).
+    Proof.
+      intros. inv H; inv H1.
+      - assert(ts = ts0 /\ rest = s).
+        {
+          apply lex_complete in H2; auto. apply lex_complete in H5; auto.
+          rewrite H2 in H5. repeat inj_all. auto.
+        }
+        destruct H. subst. clear H2 H5 rus code H0.
+        induction ts0; destruct sts; destruct sts0; try omega.
+        +  
+      - assert(ts = ts0 /\ rest = s).
+        {
+          apply lex_complete in H2; auto. apply lex_complete in H; auto.
+          rewrite H2 in H. repeat inj_all. auto.
+        }
+        destruct H1. subst. destruct Hin. destruct H1.
+        apply In_nth with (d := (defLabel, [])) in H1.
+        destruct H1. destruct H1.
+        assert(nth x0 sts defSemToken = nth x0 sts defSemToken).
+        { auto. }
+        assert(x0 < length (combine ts0 sts)).
+        { rewrite combine_length. rewrite <- H3. rewrite Nat.min_id. auto. }
+        eapply combine_nth with (n := x0) (x := (defLabel, [])) (y := defSemToken)
+          in H3.
+        eapply nth_In in H8. rewrite H3 in H8.
+        apply H4 in H8. rewrite H6 in *. rewrite H8 in *. discriminate.
+      - 
+          
+
+    Theorem lex_sem_complete : forall o code rest rus,  
+      tokenized_sem rus code o rest
+      -> rules_is_function rus 
+      -> lex_sem rus code = (o, rest).
+    Proof.
+      intros. destruct (lex_sem rus code) eqn:E.
+      eapply lex_sem_sound in E; eauto.
+      eapply tokenized_sem_unique; eauto.
+    Qed.
+        
+      
 
   End Correct.
 
